Regex/Syntax/Ast/Visitor.lean
@@ -1,4 +1,5 @@
 import Regex.Data.Array.Basic
+import Regex.Data.Array.Lemmas
 import Regex.Syntax.Ast.Ast
 
 /-!
@@ -37,237 +38,101 @@ class Visitor (α : Type v) (σ : Type w) where
 
 abbrev M σ String := StateT σ (Except String)
 
-/-- Represents a single stack frame while performing structural induction over an `Ast`.-/
-private inductive Frame where
-  | Repetition : Repetition -> Frame
-  | Group : Group -> Frame
-  | Concat : (head : Ast) -> (tail : Array Ast) -> Frame
-  | Alternation : (head : Ast) -> (tail : Array Ast) -> Frame
-
-/-- Represents a single stack frame while performing structural induction overa character class. -/
-private inductive ClassFrame where
-  /-- The stack frame used while visiting every child node of a union of character class items. -/
-  | Union (head: ClassSetItem) (tail: Array ClassSetItem) : ClassFrame
-  /-- The stack frame used while a binary class operation. -/
-  | Binary (op: ClassSetBinaryOp) : ClassFrame
-  /-- A stack frame allocated just before descending into a binary operator's
-      left hand child node. -/
-  | BinaryLHS
-        (op: ClassSetBinaryOp)
-        (lhs: ClassSet)
-        (rhs: ClassSet) : ClassFrame
-  /-- A stack frame allocated just before descending into a binary operator's
-      right hand child node. -/
-  | BinaryRHS (op: ClassSetBinaryOp) (rhs: ClassSet) : ClassFrame
-
-namespace Frame
-
-/-- Return the next child AST node to visit.-/
-private def child : Frame -> Ast
-  | .Repetition rep => rep.ast
-  | .Group g => g.ast
-  | .Concat head _ => head
-  | .Alternation head _ => head
-
-end Frame
-
-abbrev CallStack := Array (Ast × Frame)
-
-/-- A representation of the inductive step when performing structural induction . -/
-inductive ClassInduct where
-  | Item : ClassSetItem -> ClassInduct
-  | BinaryOp : ClassSetBinaryOp -> ClassInduct
-
-namespace ClassInduct
-
-def from_set : ClassSet -> ClassInduct
-  | .Item cls => ClassInduct.Item cls
-  | .BinaryOp op => ClassInduct.BinaryOp op
-
-def from_bracketed : ClassBracketed -> ClassInduct
-  | .mk _ _ cls => from_set cls
-
-end ClassInduct
-
-namespace ClassFrame
-
-def child (x : ClassFrame) : ClassInduct :=
-  match x with
-  | .Union head _ => ClassInduct.Item head
-  | .Binary op => ClassInduct.BinaryOp op
-  | .BinaryLHS _ lhs _ => ClassInduct.from_set lhs
-  | .BinaryRHS _ rhs => ClassInduct.from_set rhs
-
-end ClassFrame
-
-private def visit_class_pre {α σ: Type} (ast: ClassInduct)
+private def visit_class_pre' {α σ: Type} (ast: ClassSet)
     (β : Visitor α σ) : M σ String PUnit := do
   match ast with
-  | .Item cls => β.visit_class_set_item_pre cls
-  | .BinaryOp op => β.visit_class_set_binary_op_pre op
+  | .Item cls =>
+    β.visit_class_set_item_pre cls
+  | .BinaryOp op =>
+    β.visit_class_set_binary_op_pre op
 
-private def visit_class_post {α σ: Type} (ast: ClassInduct)
+private def visit_class_post' {α σ: Type} (ast: ClassSet)
     (β : Visitor α σ) : M σ String PUnit := do
   match ast with
-  | .Item cls => β.visit_class_set_item_post cls
-  | .BinaryOp op => β.visit_class_set_binary_op_post op
+  | .Item cls =>
+    β.visit_class_set_item_post cls
+  | .BinaryOp op =>
+    β.visit_class_set_binary_op_post op
 
-/-- Build a stack frame for the given class node -/
-private def induct_class (ast: ClassInduct) : Option ClassFrame :=
+mutual
+
+private def visit_class_item_loop' {α σ: Type} [Inhabited α]
+    (β : Visitor α σ) (item : ClassSetItem) : M σ String PUnit := do
+  β.visit_class_set_item_pre item
+  match item with
+  | .Bracketed ⟨_ , _, kind⟩  => visit_class_loop' β kind
+  | .Union ⟨_, items⟩  =>
+      items.attach.forM (fun item => do
+          have : sizeOf item.val < sizeOf items := Array.sizeOf_lt_of_mem item.property
+          visit_class_item_loop' β item.val)
+  | _ => pure ()
+  β.visit_class_set_item_post item
+termination_by sizeOf item
+
+private def visit_class_loop' {α σ: Type} [Inhabited α]
+    (β : Visitor α σ) (ast : ClassSet) : M σ String PUnit := do
+  visit_class_pre' ast β
+
   match ast with
-  | .Item (ClassSetItem.Bracketed ⟨_, _, kind⟩ ) =>
-    match kind with
-    | .Item item => some (ClassFrame.Union item #[])
-    | .BinaryOp op => some (ClassFrame.Binary op)
-  | .Item (ClassSetItem.Union union) =>
-    let ⟨_, items⟩ := union
-    if items.size = 0 then none
-    else
-      match items.head? with
-      | some (head, tail) => some (ClassFrame.Union head tail)
-      | none => none
+  | .Item (ClassSetItem.Bracketed ⟨_, _, kind⟩ ) => visit_class_loop'  β kind
+  | .Item (ClassSetItem.Union  ⟨_, items⟩) =>
+      items.attach.forM (fun item => do
+          have : sizeOf item.val < sizeOf items := Array.sizeOf_lt_of_mem item.property
+          visit_class_item_loop' β item.val)
   | .BinaryOp op =>
     match op with
-    | .mk _ _ lhs rhs => some (ClassFrame.BinaryLHS op lhs rhs)
-  | _ => none
+    | .mk _ _ lhs rhs =>
+          visit_class_loop' β lhs
+          let s ← get
+          let (_, s) ← β.visit_class_set_binary_op_in op s
+          set s
+          visit_class_loop' β rhs
+  | _ => pure ()
 
-/-- Pops the given frame. If the frame has an additional inductive step,
-    then return it, otherwise return `None`. -/
-private partial def pop_class (induct: ClassFrame) : Option ClassFrame :=
-  match induct with
-  | .Union _ tail =>
-    match tail.head? with
-    | some (head, tail) => ClassFrame.Union head tail
-    | none => none
-  | .Binary _ => none
-  | .BinaryLHS op _ rhs => ClassFrame.BinaryRHS op rhs
-  | .BinaryRHS _ _ => none
+  visit_class_post' ast β
+termination_by sizeOf ast
 
-/-- try to pop the call stack until it is either empty or hit another inductive case. -/
-private partial def visit_class_inner_loop {α σ: Type} [Inhabited α]
-    (β : Visitor α σ) (stack : Array (ClassInduct × ClassFrame))
-    : M σ String (Option ClassInduct × (Array (ClassInduct × ClassFrame))) := do
-  match Array.pop? stack with
-  | some ((post_ast, frame), stack) =>
-    match pop_class frame with
-    | some x =>
-      match x with
-      | .BinaryRHS op _ =>
-        let s ← get
-        let (_, s) ← β.visit_class_set_binary_op_in op s
-        set s
-        let stack := stack.push (post_ast, x)
-        pure (some (ClassFrame.child x), stack)
-      | _ =>
-        let stack := stack.push (post_ast, x)
-        pure (some (ClassFrame.child x), stack)
-    | none =>
-      visit_class_post post_ast β
-      visit_class_inner_loop β stack
-  | none => pure (none, #[])
-
-private partial def visit_class_loop {α σ: Type} [Inhabited α]
-    (β : Visitor α σ) (ast : ClassInduct) (stack : Array (ClassInduct × ClassFrame))
-    : M σ String PUnit := do
-  visit_class_pre ast β
-  match induct_class ast with
-  | some x =>
-    let child := ClassFrame.child x
-    let stack := stack.push (ast, x)
-    visit_class_loop β child stack
-  | none =>
-    /- No induction means we have a base case, so we can post visit it now.-/
-    visit_class_post ast β
-    match ← visit_class_inner_loop β stack with
-    | (some ast, stack) =>
-      /- Process new inductive steps. -/
-      visit_class_loop β ast stack
-    | (none, _) => pure ()
+end
 
 private def visit_class [Inhabited α] (ast: ClassBracketed)
     (β : Visitor α σ) : M σ String PUnit := do
-  let ast := ClassInduct.from_bracketed ast
-  visit_class_loop β ast #[]
+  match ast with | .mk _ _ kind => visit_class_loop' β kind
 
-/-- Build a stack frame for the given AST if one is needed-/
-private def induct [Inhabited α] (β : Visitor α σ) (ast : Ast)
-    : M σ String (Option Frame) := do
-  match ast with
-  | .ClassBracketed cls =>
-      visit_class cls β
-      pure none
-  | .Repetition rep => pure (some (Frame.Repetition rep))
-  | .Group g => pure (some (Frame.Group g))
-  | .Concat concat =>
-      match concat.asts.head? with
-      | some (head, tail) => pure (some (Frame.Concat head tail))
-      | none => pure none
-  | .Alternation ⟨_, asts⟩  =>
-      match asts.head? with
-      | some (head, tail) => pure (some (Frame.Concat head tail))
-      | none => pure none
-  | _ => pure none
-
-/-- Pops the given frame. If the frame has an additional inductive step,
-    then return it, otherwise return `None`. -/
-private def pop (induct: Frame) : Option Frame :=
-  match induct with
-  | .Repetition _ => none
-  | .Group _ => none
-  | .Concat _ tail =>
-      match tail.head? with
-      | some (head, tail) => some (Frame.Concat head tail)
-      | none => none
-  | .Alternation _ tail =>
-      match tail.head? with
-      | some (head, tail) => some (Frame.Concat head tail)
-      | none => none
-
-/- try to pop the call stack until it is either empty or we hit another inductive case.-/
-private partial def visit_inner_loop {α σ: Type} [Inhabited α]
-    (β : Visitor α σ) (stack : CallStack) : M σ String ((Option (Ast × (CallStack))) × α) := do
-  let state ← get
-  match Array.pop? stack with
-  | some ((post_ast, frame), stack) =>
-    match pop frame with
-    | some x =>
-      /- If this is a concat/alternate, then we might have additional inductive steps to process. -/
-      let ast := x.child
-      let stack := stack.push (post_ast, x)
-      pure (some (ast, stack), default)
-    | none =>
-      /- Otherwise, we've finished visiting all the child nodes, so we can post visit it now. -/
-      β.visit_post post_ast
-      visit_inner_loop β stack
-  | none =>
-    /- Call stack is empty.  -/
-    match β.finish state with
-    | Except.ok x =>
-        set state
-        pure (none, x)
-    | Except.error e => Except.error e
-
-/-- Visit every item in an `Ast` recursively -/
-partial def visit_loop {α σ: Type} [Inhabited α]
-    (β : Visitor α σ) (ast : Ast) (stack : CallStack) : M σ String α := do
+def visit_loop {α σ: Type} [Inhabited α] (β : Visitor α σ) (ast : Ast) : M σ String PUnit := do
   β.visit_pre ast
-  match ← induct β ast with
-  | some x =>
-    let child := x.child
-    let stack := stack.push (ast, x)
-    visit_loop β child stack
-  | none =>
-    /- No induction means we have a base case, so we can post visit it now.-/
-    β.visit_post ast
-    match ← visit_inner_loop β stack with
-    | (some (ast, stack), _) =>
-      /- Process new inductive steps. -/
-      visit_loop β ast stack
-    | (none, res) => pure res
+  let res ← match h : ast with
+    | .Empty | .Flags _ | .Literal _ | .Dot _ | .Assertion _ | .ClassUnicode _ | .ClassPerl _ =>
+      pure default
+    | .ClassBracketed cls =>
+      visit_class cls β
+      pure default
+    | .Repetition rep =>
+      match rep with
+      | .mk _ _ _ ast' =>
+        visit_loop β ast'
+    | .Alternation alt =>
+      match alt with
+      | .mk _ items =>
+        items.attach.forM (fun ast => do
+          have : sizeOf ast.val < sizeOf items := Array.sizeOf_lt_of_mem ast.property
+          visit_loop β ast.val)
+    | .Group g =>
+      match g with
+      | .mk _ _ ast' =>
+        visit_loop β ast'
+    | .Concat concat => do
+        have : sizeOf concat.asts < sizeOf concat := Concat.sizeOfAstsOfConcat concat
+        concat.asts.attach.forM (fun ast => do
+          have : sizeOf ast.val < sizeOf concat.asts := Array.sizeOf_lt_of_mem ast.property
+          visit_loop β ast.val)
+
+  β.visit_post ast
+  pure res
+termination_by sizeOf ast
 
 /-- Visit every item in an `Ast` recursively -/
 def visit {α σ: Type} [Inhabited α] (β : Visitor α σ) (state : σ) (ast : Ast)
     : Except String α := do
   let state := β.start state
-  let (res, _) ← visit_loop β ast default state
-  pure res
+  let (_, state) ← visit_loop β ast state
+  β.finish state
