Regex/Regex.lean
@@ -45,6 +45,7 @@ end Captures
 instance : ToString Captures where
   toString c := s!"fullMatch: {c.fullMatch}\ngroups: {c.groups}"
 
+set_option linter.dupNamespace false
 /-- A compiled regular expression for searching Unicode haystacks. -/
 structure Regex where
   nfa : Checked.NFA
@@ -83,7 +84,20 @@ private def is_overlapping_empty_match (start «end» : String.Pos) (acc : Array
       | none => false
   | none => false
 
-private partial def all_captures_loop (s : Substring) («at» : String.Pos) (re : Regex)
+theorem String.Pos.lt_def {a b : String.Pos} : a < b  ↔ a.byteIdx < b.byteIdx := Iff.rfl
+
+theorem String.Pos.sub_lt_sub_left {k m n : String.Pos} (h1 : k < m) (h2 : k < n)
+    : m - n < m - k := by
+  have : m.byteIdx - n.byteIdx < m.byteIdx - k.byteIdx := Nat.sub_lt_sub_left h1 h2
+  exact (String.Pos.lt_def.mpr this)
+
+theorem String.Pos.sizeof_lt_of_lt {a b : String.Pos} (h : a < b) : sizeOf a < sizeOf b := by
+  have sizeOf_string_pos {s : String.Pos} : sizeOf (s) = 1 + sizeOf s.byteIdx := rfl
+  apply String.Pos.lt_def.mp at h
+  rw [sizeOf_string_pos, sizeOf_string_pos, sizeOf_nat, sizeOf_nat]
+  omega
+
+private def all_captures_loop (s : Substring) («at» : String.Pos) (re : Regex)
     (logEnabled : Bool) (acc : Array String × Array Captures) : Array String × Array Captures :=
   match Log.captures s re «at» logEnabled with
   | (msgs, some captures) =>
@@ -93,10 +107,15 @@ private partial def all_captures_loop (s : Substring) («at» : String.Pos) (re 
     | some _ =>
       let overlapping_empty_match := is_overlapping_empty_match start «end» acc.2
       let next := if start = «end» then cp.next.pos else «end»
-      all_captures_loop s next re logEnabled
-        (acc.1.append msgs, (if overlapping_empty_match then acc.2 else acc.2.push captures))
+      if h : «at» < next ∧ «at» < s.stopPos then
+        have : sizeOf (s.stopPos - next) < sizeOf (s.stopPos - «at») :=
+          String.Pos.sizeof_lt_of_lt (String.Pos.sub_lt_sub_left h.right h.left)
+        all_captures_loop s next re logEnabled
+          (acc.1.append msgs, (if overlapping_empty_match then acc.2 else acc.2.push captures))
+      else (acc.1.append msgs, (if overlapping_empty_match then acc.2 else acc.2.push captures))
     | none => (acc.1.append msgs, acc.2.push captures)
   | (msgs, none) => (acc.1.append msgs, acc.2)
+termination_by s.stopPos - «at»
 
 /-- Returns an array of log msgs and all successive non-overlapping matches in the given haystack. -/
 def all_captures (s : Substring) (re : Regex) (logEnabled : Bool)
